\documentclass{tufte-handout}

\usepackage{xcolor}
\usepackage{graphicx}

% set hyperlink attributes
\hypersetup{colorlinks}

\usepackage{amsmath}

% set image attributes:
\usepackage{graphicx}
\graphicspath{ {images/} }

% create environment for bottom paragraph:
\newenvironment{bottompar}{\par\vspace*{\fill}}{\clearpage}

% ============================================================

% define the title
\title{SOC 4930/5050: Week 03 Equations Quick \\Reference}
\author{Christopher Prener, Ph.D.}
\date{September 11\textsuperscript{th}, 2017}
% ============================================================
\begin{document}
% ============================================================
\maketitle % generates the title
% ============================================================

\vspace{5mm}
\section{Median (odd \textit{n} of items)}
Let $m =$ the median item's term:
\begin{equation}
\scalebox{2} {$ m = \left( \frac { n+1 }{ 2 }  \right) ^{ th } $}
\end{equation}

\vspace{10mm}
\section{Median (even \textit{n} of items)}
\begin{subequations}
\noindent Let ${ m }_{ a } =$ the median item's term:
\begin{align}
\scalebox{2} {$ m_{ a } = \left( \frac { n+1 }{ 2 }  \right) ^{ th } $}
\end{align}

\vspace{2mm}
\noindent Let ${ x }_{ a } =$ the next lower value before ${ m }_{ a }$. Let ${ x }_{ b } =$ the next higher value after ${ m }_{ a }$.

\vspace{2mm}
\noindent Let ${ m }_{ b } =$ the median:
\begin{align}
\scalebox{2} {$ { m }_{ b } = \left( \frac { { x }_{ a } + { x }_{ b } }{ 2 } \right) $}
\end{align}
\end{subequations}

\vspace{10mm}
\section{Mean}
\begin{equation}
\scalebox{2} {$ \bar{ x } =\frac { \sum _{ i=1 }^{ n }{ x }  }{ n } $}
\end{equation}

\newpage
\section{Standard Deviation}
\begin{subequations}

\paragraph{Deviance}
\begin{equation}
\scalebox{2} {$ { D }= { (x-\bar{ x } ) } $}
\end{equation}

\vspace{3mm}
\paragraph{Total Error}
\begin{equation}
\scalebox{2} {$ { TE }= \sum _{ i=1 }^{ n }{ (x-\bar{ x } ) } $}
\end{equation}

\vspace{3mm}
\paragraph{Sum of Squared Error}
\begin{equation}
\scalebox{2} {$ { SS }= \sum _{ i=1 }^{ n }{ (x-\bar{ x } )^{ 2 } } $}
\end{equation}

\vspace{3mm}
\paragraph{Variance}
\begin{equation}
\scalebox{2} {$ { s }^{ 2 }=\frac { \sum _{ i=1 }^{ n }{ (x-\bar{ x } )^{ 2 } }  }{ n-1 } $}
\end{equation}

\vspace{3mm}
\paragraph{Standard Deviation}
\begin{equation}
\scalebox{2} {$ { s }=\sqrt { \frac { \sum _{ i=1 }^{ n }{ (x-\bar{ x } )^{ 2 } }  }{ n-1 } } $}
\end{equation}
\end{subequations}

% ============================================================
\end{document}